Sal/MRDTs/Metatheory/NegativeLedger.lean
@@ -6,6 +6,7 @@ import Sal.MRDTs.Instances.AegisSheetMaterialised
 import Sal.MRDTs.Instances.AegisSheetMaterialisedJoin
 import Sal.MRDTs.Instances.AegisSheetMaterialisedCertificates
 import Sal.MRDTs.Instances.AegisSheetMaterialisedEquivalence
+import Sal.MRDTs.Instances.AegisSheetMaterialisedUpdate
 import Sal.MRDTs.Instances.FugueMaxReplay
 import Sal.MRDTs.Metatheory.ConditioningSPOT
 import Sal.MRDTs.Metatheory.Join.Convergence_CounterModel
@@ -45,6 +46,8 @@ namespace Sal.MRDTs.Negative
 #check Instances.AegisSheet.Materialised.issuanceEstablishes
 #check Instances.AegisSheet.Materialised.replayAdequacy
 #check Instances.AegisSheet.Materialised.observationEquivalence
+#check Instances.AegisSheet.Materialised.updatePreservesCanon
+#check Instances.AegisSheet.Materialised.Reach.materialised
 #check Instances.SidedEmbedRGA.fmGeneration
 #check Instances.SidedEmbedRGA.fmReplayAdequacy
 #check Instances.SidedEmbedRGA.fuguemax_replay_witness
